freeze

src/Bedrock/End2End/X25519/EdwardsXYZT.v
@@ -53,96 +53,111 @@ Local Existing Instance field_parameters.
 Local Instance frep25519 : Field.FieldRepresentation := field_representation n Field25519.s c.
 Local Existing Instance frep25519_ok.
 
-Definition add_precomputed := func! (ox, oy, oz, ota, otb, X1, Y1, Z1, Ta1, Tb1, half_ypx, half_ymx, xyd) {
-  stackalloc 40 as YpX1;
-  fe25519_add(YpX1, Y1, X1);
-  stackalloc 40 as YmX1;
-  fe25519_sub(YmX1, Y1, X1);
-  stackalloc 40 as A;
-  fe25519_mul(A, YmX1, half_ymx);
-  stackalloc 40 as B;
-  fe25519_mul(B, YpX1, half_ypx);
-  stackalloc 40 as T1;
-  fe25519_mul(T1, Ta1, Tb1);
-  stackalloc 40 as C;
-  fe25519_mul(C, xyd, T1);
-  fe25519_sub(ota, B, A);
-  stackalloc 40 as F;
-  fe25519_sub(F, Z1, C);
-  stackalloc 40 as G;
-  fe25519_add(G, Z1, C);
-  fe25519_add(otb, B, A);
-  fe25519_mul(ox, ota, F);
-  fe25519_mul(oy, G, otb);
-  fe25519_mul(oz, F, G)
-}.
-
 Definition felem_size := Eval lazy in felem_size_in_bytes.
 
-(* Member access notation for projective points: (x, y, z, ta, tb). *)
-Local Notation "A .x" := (expr.op Syntax.bopname.add A (0)) (in custom bedrock_expr at level 2, left associativity).
-Local Notation "A .y" := (expr.op Syntax.bopname.add A (felem_size)) (in custom bedrock_expr at level 2, left associativity).
-Local Notation "A .z" := (expr.op Syntax.bopname.add A (felem_size + felem_size)) (in custom bedrock_expr at level 2, left associativity).
-Local Notation "A .ta" := (expr.op Syntax.bopname.add A (felem_size + felem_size + felem_size)) (in custom bedrock_expr at level 2, left associativity).
-Local Notation "A .tb" := (expr.op Syntax.bopname.add A (felem_size + felem_size + felem_size + felem_size)) (in custom bedrock_expr at level 2, left associativity).
+(* Projective coordinates are capitalized to avoid notation clashes. *)
+(* Member access notation for projective points: (X, Y, Z, Ta, Tb). *)
+Local Notation "A .X" := (expr.op Syntax.bopname.add A (0)) (in custom bedrock_expr at level 2, left associativity, only parsing).
+Local Notation "A .Y" := (expr.op Syntax.bopname.add A (felem_size)) (in custom bedrock_expr at level 2, left associativity, only parsing).
+Local Notation "A .Z" := (expr.op Syntax.bopname.add A (felem_size + felem_size)) (in custom bedrock_expr at level 2, left associativity, only parsing).
+Local Notation "A .Ta" := (expr.op Syntax.bopname.add A (felem_size + felem_size + felem_size)) (in custom bedrock_expr at level 2, left associativity, only parsing).
+Local Notation "A .Tb" := (expr.op Syntax.bopname.add A (felem_size + felem_size + felem_size + felem_size)) (in custom bedrock_expr at level 2, left associativity, only parsing).
+
+(* Member access notation for precomputed points: (half_ypx, half_ymx, xyd). *)
+Local Notation "A .half_ypx" := (expr.op Syntax.bopname.add A (0)) (in custom bedrock_expr at level 2, left associativity, only parsing).
+Local Notation "A .half_ymx" := (expr.op Syntax.bopname.add A (felem_size)) (in custom bedrock_expr at level 2, left associativity, only parsing).
+Local Notation "A .xyd" := (expr.op Syntax.bopname.add A (felem_size + felem_size)) (in custom bedrock_expr at level 2, left associativity, only parsing).
+
+(* Member access notation for cached points: (half_YmX, half_YpX, Z, Td). *)
+Local Notation "A .half_YmX" := (expr.op Syntax.bopname.add A (0)) (in custom bedrock_expr at level 2, left associativity, only parsing).
+Local Notation "A .half_YpX" := (expr.op Syntax.bopname.add A (felem_size)) (in custom bedrock_expr at level 2, left associativity, only parsing).
+Local Notation "A .Z" := (expr.op Syntax.bopname.add A (felem_size + felem_size)) (in custom bedrock_expr at level 2, left associativity, only parsing).
+Local Notation "A .Td" := (expr.op Syntax.bopname.add A (felem_size + felem_size + felem_size)) (in custom bedrock_expr at level 2, left associativity, only parsing).
+
+(* Adds a precomputed point p_b to projective point p_a and puts the result in p_out. *)
+Definition add_precomputed := func! (p_out, p_a, p_b) {
+  stackalloc felem_size as YpX1;
+  fe25519_add(YpX1, p_a.Y, p_a.X);
+  stackalloc felem_size as YmX1;
+  fe25519_sub(YmX1, p_a.Y, p_a.X);
+  stackalloc felem_size as A;
+  fe25519_mul(A, YmX1, p_b.half_ymx);
+  stackalloc felem_size as B;
+  fe25519_mul(B, YpX1, p_b.half_ypx);
+  stackalloc felem_size as T1;
+  fe25519_mul(T1, p_a.Ta, p_a.Tb);
+  stackalloc felem_size as C;
+  fe25519_mul(C, p_b.xyd, T1);
+  fe25519_sub(p_out.Ta, B, A);
+  stackalloc felem_size as F;
+  fe25519_sub(F, p_a.Z, C);
+  stackalloc felem_size as G;
+  fe25519_add(G, p_a.Z, C);
+  fe25519_add(p_out.Tb, B, A);
+  fe25519_mul(p_out.X, p_out.Ta, F);
+  fe25519_mul(p_out.Y, G, p_out.Tb);
+  fe25519_mul(p_out.Z, F, G)
+}.
 
 (* Equivalent of m1double in src/Curves/Edwards/XYZT/Basic.v *)
 Definition double := func! (p_out, p_a) {
   stackalloc felem_size as trX;
-  fe25519_square(trX, p_a.x);
+  fe25519_square(trX, p_a.X);
   stackalloc felem_size as trZ;
-  fe25519_square(trZ, p_a.y);
+  fe25519_square(trZ, p_a.Y);
   stackalloc felem_size as t0;
-  fe25519_square(t0, p_a.z);
+  fe25519_square(t0, p_a.Z);
   stackalloc felem_size as trT;
   fe25519_carry_add(trT, t0, t0);
   stackalloc felem_size as rY;
-  fe25519_add(rY, p_a.x, p_a.y);
+  fe25519_add(rY, p_a.X, p_a.Y);
   fe25519_square(t0, rY);
-  fe25519_carry_add(p_out.tb, trZ, trX);
+  fe25519_carry_add(p_out.Tb, trZ, trX);
   stackalloc felem_size as cZ;
   fe25519_carry_sub(cZ, trZ, trX);
-  fe25519_sub(p_out.ta, t0, p_out.tb);
+  fe25519_sub(p_out.Ta, t0, p_out.Tb);
   stackalloc felem_size as cT;
   fe25519_sub(cT, trT, cZ);
-  fe25519_mul(p_out.x, p_out.ta, cT);
-  fe25519_mul(p_out.y, p_out.tb, cZ);
-  fe25519_mul(p_out.z, cZ, cT)
+  fe25519_mul(p_out.X, p_out.Ta, cT);
+  fe25519_mul(p_out.Y, p_out.Tb, cZ);
+  fe25519_mul(p_out.Z, cZ, cT)
 }.
 
-(* Converting a normal point to a cached point to prepare it for readdition. *)
-Definition to_cached := func! (ohalf_ymx, ohalf_ypx, oz, otd, x, y, z, ta, tb, d) {
-  fe25519_sub(ohalf_ymx, y, x);
-  fe25519_half(ohalf_ymx, ohalf_ymx); (* This doesn't exist yet, work with spec for now. *)
-  fe25519_add(ohalf_ypx, y, x);
-  fe25519_half(ohalf_ypx, ohalf_ypx);
-  fe25519_mul(otd, ta, tb);
-  fe25519_mul(otd, otd, d);
-  fe25519_copy(oz, z)
+(* Converts a projective point p_a to a cached point p_out to prepare it for readdition. 
+   Uses the field's parameter d, which is passed as function argument for now. *)
+Definition to_cached := func! (p_out, p_a, p_d) {
+  fe25519_sub(p_out.half_YmX, p_a.Y, p_a.X);
+  fe25519_half(p_out.half_YmX, p_out.half_YmX); (* This doesn't exist yet, work with spec for now. *)
+  fe25519_add(p_out.half_YpX, p_a.Y, p_a.X);
+  fe25519_half(p_out.half_YpX, p_out.half_YpX);
+  fe25519_mul(p_out.Td, p_a.Ta, p_a.Tb);
+  fe25519_mul(p_out.Td, p_out.Td, p_d);
+  fe25519_copy(p_out.Z, p_a.Z)
 }.
 
-(* Equivalent of m1_readd in src/Curves/Edwards/XYZT/Readdition.v *)
-Definition readd := func! (ox, oy, oz, ota, otb, X1, Y1, Z1, Ta1, Tb1, half_YmX, half_YpX, Z2, Td) {
-  stackalloc 40 as A;
-  fe25519_sub(A, Y1, X1);
-  fe25519_mul(A, A, half_YmX);
-  stackalloc 40 as B;
-  fe25519_add(B, Y1, X1);
-  fe25519_mul(B, B, half_YpX);
-  stackalloc 40 as C;
-  fe25519_mul(C, Ta1, Tb1);
-  fe25519_mul(C, C, Td);
-  stackalloc 40 as D;
-  fe25519_mul(D, Z1, Z2);
-  fe25519_sub(ota, B, A);
-  stackalloc 40 as F;
+(* Equivalent of m1_readd in src/Curves/Edwards/XYZT/Readdition.v 
+   Adds a projective point p_a and cached point p_c and stores the result as projective point in p_out. *)
+Definition readd := func! (p_out, p_a, p_c) {
+  stackalloc felem_size as A;
+  fe25519_sub(A, p_a.Y, p_a.X);
+  fe25519_mul(A, A, p_c.half_YmX);
+  stackalloc felem_size as B;
+  fe25519_add(B, p_a.Y, p_a.X);
+  fe25519_mul(B, B, p_c.half_YpX);
+  stackalloc felem_size as C;
+  fe25519_mul(C, p_a.Ta, p_a.Tb);
+  fe25519_mul(C, C, p_c.Td);
+  stackalloc felem_size as D;
+  fe25519_mul(D, p_a.Z, p_b.Z);
+  fe25519_sub(p_out.Ta, B, A);
+  stackalloc felem_size as F;
   fe25519_sub(F, D, C);
-  stackalloc 40 as G;
+  stackalloc felem_size as G;
   fe25519_add(G, D, C);
-  fe25519_add(otb, B, A);
-  fe25519_mul(ox, ota, F);
-  fe25519_mul(oy, G, otb);
-  fe25519_mul(oz, F, G)
+  fe25519_add(p_out.Tb, B, A);
+  fe25519_mul(p_out.X, p_out.Ta, F);
+  fe25519_mul(p_out.Y, G, p_out.Tb);
+  fe25519_mul(p_out.Z, F, G)
 }.
 
 Section WithParameters.
@@ -164,7 +179,8 @@ Local Notation word := (Naive.word 32).
 Local Notation felem := (felem(FieldRepresentation:=frep25519)).
 Local Notation point := (point(Feq:=Logic.eq)(Fzero:=F.zero)(Fadd:=F.add)(Fmul:=F.mul)(a:=a)(d:=d)).
 Local Notation cached := (cached(Fzero:=F.zero)(Fadd:=F.add)(Fmul:=F.mul)(a:=a)(d:=d)).
-Local Notation coordinates := (coordinates(Feq:=Logic.eq)).
+Local Notation coordinates := (coordinates(Fzero:=F.zero)(Fadd:=F.add)(Fmul:=F.mul)(Feq:=Logic.eq)(a:=a)(d:=d)).
+Local Notation cached_coordinates := (cached_coordinates(Fzero:=F.zero)(Fadd:=F.add)(Fdiv:=F.div)(Fmul:=F.mul)(Fsub:=F.sub)(Feq:=Logic.eq)(a:=a)(d:=d)).
 Local Notation m1double :=
   (m1double(F:=F M_pos)(Feq:=Logic.eq)(Fzero:=F.zero)(Fone:=F.one)
            (Fopp:=F.opp)(Fadd:=F.add)(Fsub:=F.sub)(Fmul:=F.mul)(Finv:=F.inv)(Fdiv:=F.div)
@@ -184,6 +200,31 @@ Local Notation m1_readd :=
            (a:=a)(d:=d)(nonzero_a:=nonzero_a)(square_a:=square_a)(nonsquare_d:=nonsquare_d)
            (a_eq_minus1:=a_eq_minus1)(twice_d:=twice_d)(k_eq_2d:=k_eq_2d)(nonzero_d:=nonzero_d)).
 
+Local Notation "p .+ n" := (word.add p (word.of_Z n)) (at level 50, format "p .+ n", left associativity).
+
+(* Let's see if I can get away with one bounds config per point type. *)
+(* One problem with these is empty memory assumptions don't make that much sense anymore. *)
+
+Definition projective_repr P := { p | let '(x,y,z,ta,tb) := p in
+                            coordinates P = (feval x, feval y, feval z, feval ta, feval tb) /\
+                            bounded_by tight_bounds x /\ bounded_by tight_bounds y /\ bounded_by tight_bounds z /\
+                              bounded_by loose_bounds ta /\ bounded_by loose_bounds tb }.
+Local Notation "c '@p5@' p" := (let '(x,y,z,ta,tb) := proj1_sig c in sep (sep (sep (sep (FElem (p .+ 0) x) (FElem (p .+ 40) y)) 
+                              (FElem (p .+ 80) z)) (FElem (p .+ 120) ta)) (FElem (p .+ 160) tb)) (at level 10, format "c '@p5@' p").
+
+
+Definition precomputed_repr (P : precomputed_point) := { p | let '(half_ymx, half_ypx, xyd) := p in
+                            P = (feval half_ymx, feval half_ypx, feval xyd) /\
+                            bounded_by loose_bounds half_ymx /\ bounded_by loose_bounds half_ypx /\ bounded_by loose_bounds xyd }.
+Local Notation "c '@p3@' p" := (let '(half_ymx, half_ypx, xyd) := proj1_sig c in sep (sep (FElem (p .+ 0) half_ymx) (FElem (p .+ 40) half_ypx))
+                              (FElem (p .+ 80) xyd)) (at level 10, format "c '@p3@' p").
+
+Definition cached_repr (P : cached) := { p | let '(half_ymx, half_ypx,z,td) := p in
+                            cached_coordinates P = (feval half_ymx, feval half_ypx, feval z, feval td) /\
+                            bounded_by loose_bounds half_ymx /\ bounded_by loose_bounds half_ypx /\bounded_by loose_bounds z /\ bounded_by loose_bounds td }.
+Local Notation "c '@p4@' p" := (let '(half_ymx, half_ypx,z,td) := proj1_sig c in sep (sep (sep (FElem (p .+ 0) half_ymx) (FElem (p .+ 40) half_ypx)) (FElem (p .+ 80) z))
+                              (FElem (p .+ 120) td)) (at level 10, format "c '@p4@' p").
+
 Instance spec_of_fe25519_half : spec_of "fe25519_half" :=
   fnspec! "fe25519_half"
     (result_location input_location: word) / (old_result input: felem)
@@ -201,39 +242,16 @@ Instance spec_of_fe25519_half : spec_of "fe25519_half" :=
 
 Global Instance spec_of_add_precomputed : spec_of "add_precomputed" :=
   fnspec! "add_precomputed"
-    (oxK oyK ozK otaK otbK X1K Y1K Z1K Ta1K Tb1K half_ypxK half_ymxK xydK : word) /
-    (ox oy oz ota otb X1 Y1 Z1 Ta1 Tb1 half_ypx half_ymx xyd : felem) (R : _ -> Prop),
+    (p_out p_a p_b : word) /
+    (a : point) (b : precomputed_point) (a_repr : projective_repr a) (b_repr : precomputed_repr b) (R : _ -> Prop),
   { requires t m :=
-      bounded_by tight_bounds X1 /\
-      bounded_by tight_bounds Y1 /\
-      bounded_by tight_bounds Z1 /\
-      bounded_by loose_bounds Ta1 /\
-      bounded_by loose_bounds Tb1 /\
-      bounded_by loose_bounds half_ypx /\
-      bounded_by loose_bounds half_ymx /\
-      bounded_by loose_bounds xyd /\
-      m =* (FElem X1K X1) * (FElem Y1K Y1) * (FElem Z1K Z1) * (FElem Ta1K Ta1) * (FElem Tb1K Tb1) * (FElem half_ypxK half_ypx) * (FElem half_ymxK half_ymx) * (FElem xydK xyd) * (FElem oxK ox) * (FElem oyK oy) * (FElem ozK oz) * (FElem otaK ota) * (FElem otbK otb) * R;
+      m =* a_repr @p5@ p_a * b_repr @p3@ p_b * R;  (* TODO memory for p_out *) 
     ensures t' m' :=
       t = t' /\
-      exists ox' oy' oz' ota' otb',
-        ((feval ox'), (feval oy'), (feval oz'), (feval ota'), (feval otb')) = (@m1add_precomputed_coordinates (F M_pos) (F.add) (F.sub) (F.mul) ((feval X1), (feval Y1), (feval Z1), (feval Ta1), (feval Tb1)) ((feval half_ypx), (feval half_ymx), (feval xyd))) /\
-        bounded_by loose_bounds ox' /\
-        bounded_by loose_bounds oy' /\
-        bounded_by loose_bounds oz' /\
-        bounded_by loose_bounds ota' /\
-        bounded_by loose_bounds otb' /\
-        m' =* (FElem X1K X1) * (FElem Y1K Y1) * (FElem Z1K Z1) * (FElem Ta1K Ta1) * (FElem Tb1K Tb1) * (FElem half_ypxK half_ypx) * (FElem half_ymxK half_ymx) * (FElem xydK xyd) * (FElem oxK ox') * (FElem oyK oy') * (FElem ozK oz') * (FElem otaK ota') * (FElem otbK otb') * R }.
-
-Definition point_repr_bounds := (Field.bounds * Field.bounds * Field.bounds * Field.bounds * Field.bounds)%type.
-Definition point_repr := (felem * felem * felem * felem * felem)%type.
-Definition feval_point_repr '(x, y, z, ta, tb) := (feval x, feval y, feval z, feval ta, feval tb).
-
-Definition point_repr_bounded_by (bounds : point_repr_bounds) '(x,y,z,ta,tb) : Prop :=
-  let '(bounds_x, bounds_y, bounds_z, bounds_ta, bounds_tb) := bounds in
-  bounded_by bounds_x x /\ bounded_by bounds_y y /\ bounded_by bounds_z z /\ bounded_by bounds_ta ta /\ bounded_by bounds_tb tb.
-
-Local Notation "p .+ n" := (word.add p (word.of_Z n)) (at level 50, format "p .+ n", left associativity).
-Local Notation "c p@ p" := (let '(x,y,z,ta,tb) := c in sep (sep (sep (sep (FElem (p .+ 0) x) (FElem (p .+ 40) y)) (FElem (p .+ 80) z)) (FElem (p .+ 120) ta)) (FElem (p .+ 160) tb)) (at level 10, format "c p@ p").
+      (* Oof, I am starting to remember why I disliked using sigma types, you just start pulling your props into your type. 
+         Now the fact that p_out is the right output point suddenly depends on the fact that m1add_ is on the curve. *)
+      exists p_out : projective_repr (m1add_precomputed_coordinates (coordinates a) b), (* Probably need to tighten bounds for this to work... *)
+        m' =* a_repr @p5@ p_a * b @p3@ p_b * R }.
 
 Global Instance spec_of_double : spec_of "double" :=
   fnspec! "double"
@@ -465,6 +483,7 @@ Proof.
   destruct p as (((((x, y), z), ta), tb), HP).
   destruct anything as ((((ax, ay), az), ata), atb).
   lazy beta match delta [point_repr_bounded_by feval_point_repr coordinates proj1_sig] in *.
+  cbv beta match delta [point_repr_bounded_by feval_point_repr coordinates proj1_sig] in *.
   repeat straightline.
   inversion H13.
   repeat single_step.
